Revise Lib.IntTypes
- restrict add_mod, sub_mod, and mul_mod to unsigned operators
- avoid using mathematical integers in definitions meant to be extracted
- remove unnecessary integer type restrictions in a few lemmas
- implement div and mod for signed types and prove respective lemmas
- remove admits
- remove unused definitions shift_right_negative (use shift_right_arithmetic), shift_left_negative (unextractable)

lib/Lib.IntTypes.fst
@@ -4,9 +4,10 @@ open FStar.Math.Lemmas
 
 #push-options "--max_fuel 0 --max_ifuel 1 --z3rlimit 50"
 
-let pow2_2 _ = assert_norm (pow2 2 = 4)
-let pow2_3 _ = assert_norm (pow2 3 = 8)
-let pow2_4 _ = assert_norm (pow2 4 = 16)
+let pow2_2 _   = assert_norm (pow2 2 = 4)
+let pow2_3 _   = assert_norm (pow2 3 = 8)
+let pow2_4 _   = assert_norm (pow2 4 = 16)
+let pow2_127 _ = assert_norm (pow2 127 = 0x80000000000000000000000000000000)
 
 let sec_int_t t = pub_int_t t
 
@@ -57,184 +58,199 @@ let v_mk_int #t #l n = ()
 
 let size_to_uint32 x = x
 
-let size_to_uint64 x = FStar.Int.Cast.uint32_to_uint64 x
+let size_to_uint64 x = Int.Cast.uint32_to_uint64 x
 
 let byte_to_uint8 x = x
 
-let byte_to_int8 x = FStar.Int.Cast.uint8_to_int8 x
+let byte_to_int8 x = Int.Cast.uint8_to_int8 x
 
-#push-options "--z3rlimit 200"
+#push-options "--z3rlimit 300"
+
+let op_At_Percent = Int.op_At_Percent
+
+// FStar.UInt128 gets special treatment in KreMLin 
+// There is no equivalent for FStar.Int128 at the moment, so we assume
+// these casts for the time being. Using them will fail at runtime with 
+// an informative message. The commented-out implementations show that they
+// are realizable.
+
+// U1,U8,U16,U32,U64 -> S128
+assume 
+val uint64_to_int128: a:UInt64.t -> b:Int128.t{Int128.v b == UInt64.v a}
+//let uint64_to_int128 a = Int128.int_to_t (v a)
+
+// U128 -> S128
+assume 
+val uint128_to_int128: a:UInt128.t{v a <= maxint S128} -> b:Int128.t{Int128.v b == UInt128.v a}
+//let uint128_to_int128 a = Int128.int_to_t (v a)
+
+// S8,S16,S32,S64 -> S128
+assume 
+val int64_to_int128: a:Int64.t -> b:Int128.t{Int128.v b == Int64.v a}
+//let int64_to_int128 a = Int128.int_to_t (v a)
+
+// S8,S16,S32,S64 -> U128
+assume 
+val int64_to_uint128: a:Int64.t -> b:UInt128.t{UInt128.v b == Int64.v a % pow2 128}
+//let int64_to_uint128 a = mk_int (v a % pow2 128)
+
+// S128 -> U128
+assume 
+val int128_to_uint128: a:Int128.t -> b:UInt128.t{UInt128.v b == Int128.v a % pow2 128}
+//let int128_to_uint128 a = mk_int (v a % pow2 128)
+
+// S128 -> U1..U64,S8..S64
+assume
+val int128_to_uint64: a:Int128.t -> b:UInt64.t{UInt64.v b == Int128.v a % pow2 64}
+//let int128_to_uint64 a = UInt64.uint_to_t (v a % pow2 64)
 
 let cast #t #l t' l' u =
-  assert_norm (pow2 8 = 2 * pow2 7); 
-  assert_norm (pow2 16 = 2 * pow2 15); 
-  assert_norm (pow2 128 = 2 * pow2 127); 
+  assert_norm (pow2 8 = 2 * pow2 7);
+  assert_norm (pow2 16 = 2 * pow2 15);
+  assert_norm (pow2 64 * pow2 64 = pow2 128);
+  assert_norm (pow2 16 * pow2 48 = pow2 64);
+  assert_norm (pow2 8 * pow2 56 = pow2 64);
+  assert_norm (pow2 32 * pow2 32 = pow2 64);
+  modulo_modulo_lemma (v u) (pow2 32) (pow2 32);
+  modulo_modulo_lemma (v u) (pow2 64) (pow2 64);
+  modulo_modulo_lemma (v u) (pow2 128) (pow2 64);
+  modulo_modulo_lemma (v u) (pow2 16) (pow2 48);
+  modulo_modulo_lemma (v u) (pow2 8) (pow2 56);
   let open FStar.Int.Cast in
+  let open FStar.Int.Cast.Full in
   match t, t' with
-  | U1, U1 -> u
-  | U1, U8 -> u
-  | U1, U16 -> uint8_to_uint16 u
-  | U1, U32 -> uint8_to_uint32 u
-  | U1, U64 -> uint8_to_uint64 u
-  | U1, U128 -> UInt128.uint64_to_uint128 (uint8_to_uint64 u)
-  | U1, S8 -> uint8_to_int8 u
-  | U1, S16 -> uint8_to_int16 u
-  | U1, S32 -> uint8_to_int32 u
-  | U1, S64 -> uint8_to_int64 u
-  | U1, S128 -> pow2_le_compat (bits t' - 1) (bits t); mk_int #S128 #l' (v u)
+  | U1, U1     -> u
+  | U1, U8     -> u
+  | U1, U16    -> uint8_to_uint16 u
+  | U1, U32    -> uint8_to_uint32 u
+  | U1, U64    -> uint8_to_uint64 u
+  | U1, U128   -> UInt128.uint64_to_uint128 (uint8_to_uint64 u)
+  | U1, S8     -> uint8_to_int8 u
+  | U1, S16    -> uint8_to_int16 u
+  | U1, S32    -> uint8_to_int32 u
+  | U1, S64    -> uint8_to_int64 u
+  | U1, S128   -> uint64_to_int128 (uint8_to_uint64 u)
 
-  | U8, U1 -> UInt8.rem u 2uy
-  | U8, U8 -> u
-  | U8, U16 -> uint8_to_uint16 u
-  | U8, U32 -> uint8_to_uint32 u
-  | U8, U64 -> uint8_to_uint64 u
-  | U8, U128 -> UInt128.uint64_to_uint128 (uint8_to_uint64 u)
-  | U8, S8 -> uint8_to_int8 u
-  | U8, S16 -> uint8_to_int16 u
-  | U8, S32 -> uint8_to_int32 u
-  | U8, S64 -> uint8_to_int64 u
-  | U8, S128 -> pow2_le_compat (bits t' - 1) (bits t); mk_int #S128 #l' (v u)
+  | U8, U1     -> UInt8.rem u 2uy
+  | U8, U8     -> u
+  | U8, U16    -> uint8_to_uint16 u
+  | U8, U32    -> uint8_to_uint32 u
+  | U8, U64    -> uint8_to_uint64 u
+  | U8, U128   -> UInt128.uint64_to_uint128 (uint8_to_uint64 u)
+  | U8, S8     -> uint8_to_int8 u
+  | U8, S16    -> uint8_to_int16 u
+  | U8, S32    -> uint8_to_int32 u
+  | U8, S64    -> uint8_to_int64 u
+  | U8, S128   -> uint64_to_int128 (uint8_to_uint64 u)
 
-  | U16, U1 -> uint16_to_uint8 (UInt16.rem u 2us)
-  | U16, U8 -> uint16_to_uint8 u
-  | U16, U16 -> u
-  | U16, U32 -> uint16_to_uint32 u
-  | U16, U64 -> uint16_to_uint64 u
-  | U16, U128 -> UInt128.uint64_to_uint128 (uint16_to_uint64 u)
-  | U16, S8 -> uint16_to_int8 u
-  | U16, S16 -> uint16_to_int16 u
-  | U16, S32 -> uint16_to_int32 u
-  | U16, S64 -> uint16_to_int64 u
-  | U16, S128 -> pow2_le_compat (bits t' - 1) (bits t); mk_int #S128 #l' (v u)
-  
-  | U32, U1 -> uint32_to_uint8 (UInt32.rem u 2ul)
-  | U32, U8 -> uint32_to_uint8 u
-  | U32, U16 -> uint32_to_uint16 u
-  | U32, U32 -> u
-  | U32, U64 -> uint32_to_uint64 u
-  | U32, U128 -> UInt128.uint64_to_uint128 (uint32_to_uint64 u)
-  | U32, S8 -> uint32_to_int8 u
-  | U32, S16 -> uint32_to_int16 u
-  | U32, S32 -> uint32_to_int32 u
-  | U32, S64 -> uint32_to_int64 u
-  | U32, S128 -> pow2_le_compat (bits t' - 1) (bits t); mk_int #S128 #l' (v u)
-  
-  | U64, U1 -> uint64_to_uint8 (UInt64.rem u 2uL)
-  | U64, U8 -> uint64_to_uint8 u
-  | U64, U16 -> uint64_to_uint16 u
-  | U64, U32 -> uint64_to_uint32 u
-  | U64, U64 -> u
-  | U64, U128 -> UInt128.uint64_to_uint128 u
-  | U64, S8 -> uint64_to_int8 u
-  | U64, S16 -> uint64_to_int16 u
-  | U64, S32 -> uint64_to_int32 u
-  | U64, S64 -> uint64_to_int64 u
-  | U64, S128 -> pow2_le_compat (bits t' - 1) (bits t); mk_int #S128 #l' (v u)
+  | U16, U1    -> UInt8.rem (uint16_to_uint8 u) 2uy
+  | U16, U8    -> uint16_to_uint8 u
+  | U16, U16   -> u
+  | U16, U32   -> uint16_to_uint32 u
+  | U16, U64   -> uint16_to_uint64 u
+  | U16, U128  -> UInt128.uint64_to_uint128 (uint16_to_uint64 u)
+  | U16, S8    -> uint16_to_int8 u
+  | U16, S16   -> uint16_to_int16 u
+  | U16, S32   -> uint16_to_int32 u
+  | U16, S64   -> uint16_to_int64 u
+  | U16, S128  -> uint64_to_int128 (uint16_to_uint64 u)
 
-  | U128, U1 ->
-    assert_norm (pow2 64 * pow2 64 = pow2 128);
-    assert_norm (pow2 8 * pow2 56 = pow2 64);
-    modulo_modulo_lemma (v u) (pow2 64) (pow2 64);
-    modulo_modulo_lemma (v u) (pow2 8) (pow2 56);
-    UInt8.rem (uint64_to_uint8 (FStar.Int.Cast.Full.uint128_to_uint64 u)) 0x2uy
-  | U128, U8 ->
-    assert_norm (pow2 64 * pow2 64 = pow2 128);
-    assert_norm (pow2 8 * pow2 56 = pow2 64);
-    modulo_modulo_lemma (v u) (pow2 64) (pow2 64);
-    modulo_modulo_lemma (v u) (pow2 8) (pow2 56);
-    uint64_to_uint8 (UInt128.uint128_to_uint64 u)
-  | U128, U16 ->
-    assert_norm (pow2 64 * pow2 64 = pow2 128);
-    assert_norm (pow2 16 * pow2 48 = pow2 64);
-    modulo_modulo_lemma (v u) (pow2 64) (pow2 64);
-    modulo_modulo_lemma (v u) (pow2 16) (pow2 48);
-    uint64_to_uint16 (UInt128.uint128_to_uint64 u)
-  | U128, U32 ->
-    assert_norm (pow2 64 * pow2 64 = pow2 128);
-    assert_norm (pow2 32 * pow2 32 = pow2 64);
-    modulo_modulo_lemma (v u) (pow2 64) (pow2 64);
-    modulo_modulo_lemma (v u) (pow2 32) (pow2 32);
-    uint64_to_uint32 (UInt128.uint128_to_uint64 u)
-  | U128, U64 ->
-    assert_norm (pow2 64 * pow2 64 = pow2 128);
-    modulo_modulo_lemma (v u) (pow2 64) (pow2 64);
-    UInt128.uint128_to_uint64 u
+  | U32, U1    -> UInt8.rem (uint32_to_uint8 u) 2uy
+  | U32, U8    -> uint32_to_uint8 u
+  | U32, U16   -> uint32_to_uint16 u
+  | U32, U32   -> u
+  | U32, U64   -> uint32_to_uint64 u
+  | U32, U128  -> UInt128.uint64_to_uint128 (uint32_to_uint64 u)
+  | U32, S8    -> uint32_to_int8 u
+  | U32, S16   -> uint32_to_int16 u
+  | U32, S32   -> uint32_to_int32 u
+  | U32, S64   -> uint32_to_int64 u
+  | U32, S128  -> uint64_to_int128 (uint32_to_uint64 u)
+
+  | U64, U1    -> UInt8.rem (uint64_to_uint8 u) 2uy
+  | U64, U8    -> uint64_to_uint8 u
+  | U64, U16   -> uint64_to_uint16 u
+  | U64, U32   -> uint64_to_uint32 u
+  | U64, U64   -> u
+  | U64, U128  -> UInt128.uint64_to_uint128 u
+  | U64, S8    -> uint64_to_int8 u
+  | U64, S16   -> uint64_to_int16 u
+  | U64, S32   -> uint64_to_int32 u
+  | U64, S64   -> uint64_to_int64 u
+  | U64, S128  -> uint64_to_int128 u
+
+  | U128, U1   -> UInt8.rem (uint64_to_uint8 (uint128_to_uint64 u)) 2uy
+  | U128, U8   -> uint64_to_uint8 (UInt128.uint128_to_uint64 u)
+  | U128, U16  -> uint64_to_uint16 (UInt128.uint128_to_uint64 u)
+  | U128, U32  -> uint64_to_uint32 (UInt128.uint128_to_uint64 u)
+  | U128, U64  -> UInt128.uint128_to_uint64 u
   | U128, U128 -> u
-  | U128, S8 ->
-    assert_norm (pow2 64 * pow2 64 = pow2 128);
-    assert_norm (pow2 8 * pow2 56 = pow2 64);
-    modulo_modulo_lemma (v u) (pow2 64) (pow2 64);
-    modulo_modulo_lemma (v u) (pow2 8) (pow2 56);
-    uint64_to_int8 (UInt128.uint128_to_uint64 u)
-  | U128, S16 ->
-    assert_norm (pow2 64 * pow2 64 = pow2 128);
-    assert_norm (pow2 16 * pow2 48 = pow2 64);
-    modulo_modulo_lemma (v u) (pow2 64) (pow2 64);
-    modulo_modulo_lemma (v u) (pow2 16) (pow2 48);
-    uint64_to_int16 (UInt128.uint128_to_uint64 u)
-  | U128, S32 ->
-    assert_norm (pow2 64 * pow2 64 = pow2 128);
-    assert_norm (pow2 32 * pow2 32 = pow2 64);
-    modulo_modulo_lemma (v u) (pow2 64) (pow2 64);
-    modulo_modulo_lemma (v u) (pow2 32) (pow2 32);
-    uint64_to_int32 (UInt128.uint128_to_uint64 u)
-  | U128, S64 ->
-    assert_norm (pow2 64 * pow2 64 = pow2 128);
-    modulo_modulo_lemma (v u) (pow2 64) (pow2 64);
-    uint64_to_int64 (UInt128.uint128_to_uint64 u)
-  | U128, S128 -> assert_norm (pow2 128 = 2 * pow2 127); mk_int #S128 #l' (v u @%. t')
+  | U128, S8   -> uint64_to_int8 (UInt128.uint128_to_uint64 u)
+  | U128, S16  -> uint64_to_int16 (UInt128.uint128_to_uint64 u)
+  | U128, S32  -> uint64_to_int32 (UInt128.uint128_to_uint64 u)
+  | U128, S64  -> uint64_to_int64 (UInt128.uint128_to_uint64 u)
+  | U128, S128 -> uint128_to_int128 u
 
-  | S8, U1 -> UInt8.rem (int8_to_uint8 u) 2uy
-  | S8, U8 -> int8_to_uint8 u
-  | S8, U16 -> int8_to_uint16 u
-  | S8, U32 -> int8_to_uint32 u
-  | S8, U64 -> int8_to_uint64 u
-  | S8, U128 -> pow2_le_compat (bits t') (bits t - 1); mk_int #U128 #l' (v u % modulus U128)
-  | S8, S8 ->  u
-  | S8, S16 -> int8_to_int16 u
-  | S8, S32 -> int8_to_int32 u
-  | S8, S64 -> int8_to_int64 u
-  | S8, S128 -> pow2_le_compat (bits t' - 1) (bits t - 1); mk_int #S128 #l' (v u)
+  | S8, U1     -> UInt8.rem (int8_to_uint8 u) 2uy
+  | S8, U8     -> int8_to_uint8 u
+  | S8, U16    -> int8_to_uint16 u
+  | S8, U32    -> int8_to_uint32 u
+  | S8, U64    -> int8_to_uint64 u
+  | S8, U128   -> int64_to_uint128 (int8_to_int64 u)
+  | S8, S8     -> u
+  | S8, S16    -> int8_to_int16 u
+  | S8, S32    -> int8_to_int32 u
+  | S8, S64    -> int8_to_int64 u   
+  | S8, S128   -> int64_to_int128 (int8_to_int64 u) 
 
-  | S16, U1 -> UInt8.rem (int16_to_uint8 u) 2uy
-  | S16, U8 -> int16_to_uint8 u
-  | S16, U16 -> int16_to_uint16 u
-  | S16, U32 -> int16_to_uint32 u
-  | S16, U64 -> int16_to_uint64 u
-  | S16, U128 -> pow2_le_compat (bits t') (bits t - 1); mk_int #U128 #l' (v u % modulus U128)
-  | S16, S8 -> int16_to_int8 u
-  | S16, S16 -> u
-  | S16, S32 -> int16_to_int32 u
-  | S16, S64 -> int16_to_int64 u
-  | S16, S128 -> pow2_le_compat (bits t' - 1) (bits t - 1); mk_int #S128 #l' (v u)
+  | S16, U1    -> UInt8.rem (int16_to_uint8 u) 2uy
+  | S16, U8    -> int16_to_uint8 u
+  | S16, U16   -> int16_to_uint16 u
+  | S16, U32   -> int16_to_uint32 u
+  | S16, U64   -> int16_to_uint64 u
+  | S16, U128  -> int64_to_uint128 (int16_to_int64 u)
+  | S16, S8    -> int16_to_int8 u
+  | S16, S16   -> u
+  | S16, S32   -> int16_to_int32 u
+  | S16, S64   -> int16_to_int64 u
+  | S16, S128  -> int64_to_int128 (int16_to_int64 u)
+
+  | S32, U1    -> UInt8.rem (int32_to_uint8 u) 2uy
+  | S32, U8    -> int32_to_uint8 u
+  | S32, U16   -> int32_to_uint16 u
+  | S32, U32   -> int32_to_uint32 u
+  | S32, U64   -> int32_to_uint64 u
+  | S32, U128  -> int64_to_uint128 (int32_to_int64 u)
+  | S32, S8    -> int32_to_int8 u
+  | S32, S16   -> int32_to_int16 u
+  | S32, S32   -> u
+  | S32, S64   -> int32_to_int64 u
+  | S32, S128  -> int64_to_int128 (int32_to_int64 u)
+
+  | S64, U1    -> UInt8.rem (int64_to_uint8 u) 2uy
+  | S64, U8    -> int64_to_uint8 u
+  | S64, U16   -> int64_to_uint16 u
+  | S64, U32   -> int64_to_uint32 u
+  | S64, U64   -> int64_to_uint64 u
+  | S64, U128  -> int64_to_uint128 u
+  | S64, S8    -> int64_to_int8 u
+  | S64, S16   -> int64_to_int16 u
+  | S64, S32   -> int64_to_int32 u
+  | S64, S64   -> u
+  | S64, S128  -> int64_to_int128 u
+
+  | S128, U1    -> UInt8.rem (uint64_to_uint8 (int128_to_uint64 u)) 2uy  
+  | S128, U8    -> uint64_to_uint8 (int128_to_uint64 u)
+  | S128, U16   -> uint64_to_uint16 (int128_to_uint64 u)
+  | S128, U32   -> uint64_to_uint32 (int128_to_uint64 u)
+  | S128, U64   -> int128_to_uint64 u  
+  | S128, U128  -> int128_to_uint128 u
+  | S128, S8    -> uint64_to_int8  (int128_to_uint64 u)
+  | S128, S16   -> uint64_to_int16 (int128_to_uint64 u)
+  | S128, S32   -> uint64_to_int32 (int128_to_uint64 u)
+  | S128, S64   -> uint64_to_int64 (int128_to_uint64 u)
+  | S128, S128  -> u
   
-  | S32, U1 -> UInt8.rem (int32_to_uint8 u) 2uy
-  | S32, U8 -> int32_to_uint8 u
-  | S32, U16 -> int32_to_uint16 u
-  | S32, U32 -> int32_to_uint32 u
-  | S32, U64 -> int32_to_uint64 u
-  | S32, U128 -> pow2_le_compat (bits t') (bits t - 1); mk_int #U128 #l' (v u % modulus U128)
-  | S32, S8 -> int32_to_int8 u
-  | S32, S16 -> int32_to_int16 u
-  | S32, S32 -> u
-  | S32, S64 -> int32_to_int64 u
-  | S32, S128 -> pow2_le_compat (bits t' - 1) (bits t - 1); mk_int #S128 #l' (v u)
-
-  | S64, U1 -> UInt8.rem (int64_to_uint8 u) 2uy
-  | S64, U8 -> int64_to_uint8 u
-  | S64, U16 -> int64_to_uint16 u
-  | S64, U32 -> int64_to_uint32 u
-  | S64, U64 -> int64_to_uint64 u
-  | S64, U128 -> pow2_le_compat (bits t') (bits t - 1); mk_int #U128 #l' (v u % modulus U128)
-  | S64, S8 -> int64_to_int8 u
-  | S64, S16 -> int64_to_int16 u
-  | S64, S32 -> int64_to_int32 u
-  | S64, S64 -> u
-  | S64, S128 -> pow2_le_compat (bits t' - 1) (bits t - 1); mk_int #S128 #l' (v u)
-  
-  | S128, S128 -> u
-  | S128, _ -> mk_int #t' #l' (v u @%. t')
-
 #pop-options
 
 let ones t l = mk_int #t #l (ones_v t)
@@ -249,11 +265,6 @@ let add_mod #t #l a b =
   | U32  -> UInt32.add_mod a b
   | U64  -> UInt64.add_mod a b
   | U128 -> UInt128.add_mod a b
-  | S8   -> Int8.int_to_t (Int.add_mod (Int8.v a) (Int8.v b))
-  | S16  -> Int16.int_to_t (Int.add_mod (Int16.v a) (Int16.v b))
-  | S32  -> Int32.int_to_t (Int.add_mod (Int32.v a) (Int32.v b))
-  | S64  -> Int64.int_to_t (Int.add_mod (Int64.v a) (Int64.v b))
-  | S128 -> Int128.int_to_t (Int.add_mod (Int128.v a) (Int128.v b))
 
 let add_mod_lemma #t #l a b = ()
 
@@ -265,28 +276,28 @@ let add #t #l a b =
   | U32  -> UInt32.add a b
   | U64  -> UInt64.add a b
   | U128 -> UInt128.add a b
-  | S8 -> Int8.add a b
-  | S16 -> Int16.add a b
-  | S32 -> Int32.add a b
-  | S64 -> Int64.add a b
+  | S8   -> Int8.add a b
+  | S16  -> Int16.add a b
+  | S32  -> Int32.add a b
+  | S64  -> Int64.add a b
   | S128 -> Int128.add a b
-  
+
 let add_lemma #t #l a b = ()
 
 #push-options "--max_fuel 1"
 
 let incr #t #l a =
   match t with
-  | U1   -> UInt8.add a 0x1uy
-  | U8   -> UInt8.add a 0x1uy
-  | U16  -> UInt16.add a 0x1us
-  | U32  -> UInt32.add a 0x1ul
-  | U64  -> UInt64.add a 0x1uL
+  | U1   -> UInt8.add a 1uy
+  | U8   -> UInt8.add a 1uy
+  | U16  -> UInt16.add a 1us
+  | U32  -> UInt32.add a 1ul
+  | U64  -> UInt64.add a 1uL
   | U128 -> UInt128.add a (UInt128.uint_to_t 1)
-  | S8 -> Int8.add a 0x1y
-  | S16 -> Int16.add a 0x1s
-  | S32 -> Int32.add a 0x1l
-  | S64 -> Int64.add a 0x1L
+  | S8   -> Int8.add a 1y
+  | S16  -> Int16.add a 1s
+  | S32  -> Int32.add a 1l
+  | S64  -> Int64.add a 1L
   | S128 -> Int128.add a (Int128.int_to_t 1)
 
 let incr_lemma #t #l a = ()
@@ -300,11 +311,7 @@ let mul_mod #t #l a b =
   | U16 -> UInt16.mul_mod a b
   | U32 -> UInt32.mul_mod a b
   | U64 -> UInt64.mul_mod a b
-  | S8 -> Int8.int_to_t (Int.mul_mod (Int8.v a) (Int8.v b))
-  | S16 -> Int16.int_to_t (Int.mul_mod (Int16.v a) (Int16.v b))
-  | S32 -> Int32.int_to_t (Int.mul_mod (Int32.v a) (Int32.v b))
-  | S64 -> Int64.int_to_t (Int.mul_mod (Int64.v a) (Int64.v b))
-  
+
 let mul_mod_lemma #t #l a b = ()
 
 let mul #t #l a b =
@@ -314,11 +321,11 @@ let mul #t #l a b =
   | U16 -> UInt16.mul a b
   | U32 -> UInt32.mul a b
   | U64 -> UInt64.mul a b
-  | S8 -> Int8.mul a b
+  | S8  -> Int8.mul a b
   | S16 -> Int16.mul a b
   | S32 -> Int32.mul a b
   | S64 -> Int64.mul a b
-  
+
 let mul_lemma #t #l a b = ()
 
 let mul64_wide a b = UInt128.mul_wide a b
@@ -331,17 +338,12 @@ let mul_s64_wide_lemma a b = ()
 
 let sub_mod #t #l a b =
   match t with
-  | U1   -> UInt8.rem (UInt8.sub_mod a b) 0x2uy
+  | U1   -> UInt8.rem (UInt8.sub_mod a b) 2uy
   | U8   -> UInt8.sub_mod a b
   | U16  -> UInt16.sub_mod a b
   | U32  -> UInt32.sub_mod a b
   | U64  -> UInt64.sub_mod a b
   | U128 -> UInt128.sub_mod a b
-  | S8 -> Int8.int_to_t (Int.sub_mod (Int8.v a) (Int8.v b))
-  | S16 -> Int16.int_to_t (Int.sub_mod (Int16.v a) (Int16.v b))
-  | S32 -> Int32.int_to_t (Int.sub_mod (Int32.v a) (Int32.v b))
-  | S64 -> Int64.int_to_t (Int.sub_mod (Int64.v a) (Int64.v b))
-  | S128 -> Int128.int_to_t (Int.sub_mod (Int128.v a) (Int128.v b))
 
 let sub_mod_lemma #t #l a b = ()
 
@@ -353,28 +355,28 @@ let sub #t #l a b =
   | U32  -> UInt32.sub a b
   | U64  -> UInt64.sub a b
   | U128 -> UInt128.sub a b
-  | S8 -> Int8.sub a b
-  | S16 -> Int16.sub a b
-  | S32 -> Int32.sub a b
-  | S64 -> Int64.sub a b
+  | S8   -> Int8.sub a b
+  | S16  -> Int16.sub a b
+  | S32  -> Int32.sub a b
+  | S64  -> Int64.sub a b
   | S128 -> Int128.sub a b
-  
+
 let sub_lemma #t #l a b = ()
 
 #push-options "--max_fuel 1"
 
 let decr #t #l a =
   match t with
-  | U1   -> UInt8.sub a 0x1uy
-  | U8   -> UInt8.sub a 0x1uy
-  | U16  -> UInt16.sub a 0x1us
-  | U32  -> UInt32.sub a 0x1ul
-  | U64  -> UInt64.sub a 0x1uL
+  | U1   -> UInt8.sub a 1uy
+  | U8   -> UInt8.sub a 1uy
+  | U16  -> UInt16.sub a 1us
+  | U32  -> UInt32.sub a 1ul
+  | U64  -> UInt64.sub a 1uL
   | U128 -> UInt128.sub a (UInt128.uint_to_t 1)
-  | S8   -> Int8.sub a 0x1y
-  | S16  -> Int16.sub a 0x1s
-  | S32  -> Int32.sub a 0x1l
-  | S64  -> Int64.sub a 0x1L
+  | S8   -> Int8.sub a 1y
+  | S16  -> Int16.sub a 1s
+  | S32  -> Int32.sub a 1l
+  | S64  -> Int64.sub a 1L
   | S128 -> Int128.sub a (Int128.int_to_t 1)
 
 let decr_lemma #t #l a = ()
@@ -399,38 +401,38 @@ let logxor #t #l a b =
   | S32  -> Int32.logxor a b
   | S64  -> Int64.logxor a b
   | S128 -> Int128.logxor a b
-  
-#push-options "--max_fuel 1" 
+
+#push-options "--max_fuel 1"
 
 val logxor_lemma_: #t:inttype -> #l:secrecy_level -> a:int_t t l -> b:int_t t l -> Lemma
   (v (a `logxor` (a `logxor` b)) == v b)
 let logxor_lemma_ #t #l a b =
   match t with
-  | U1 |U8 |U16 |U32 |U64 |U128 ->
-  UInt.logxor_associative #(bits t) (v a) (v a) (v b);
-  UInt.logxor_self #(bits t) (v a);
-  UInt.logxor_commutative #(bits t) 0 (v b);
-  UInt.logxor_lemma_1 #(bits t) (v b)
-  | S8 |S16 |S32 |S64 |S128 ->
-  Int.logxor_associative #(bits t) (v a) (v a) (v b);
-  Int.logxor_self #(bits t) (v a);
-  Int.logxor_commutative #(bits t) 0 (v b);
-  Int.logxor_lemma_1 #(bits t) (v b)
+  | U1 | U8 | U16 | U32 | U64 | U128 ->
+    UInt.logxor_associative #(bits t) (v a) (v a) (v b);
+    UInt.logxor_self #(bits t) (v a);
+    UInt.logxor_commutative #(bits t) 0 (v b);
+    UInt.logxor_lemma_1 #(bits t) (v b)
+  | S8 | S16 | S32 | S64 | S128 ->
+    Int.logxor_associative #(bits t) (v a) (v a) (v b);
+    Int.logxor_self #(bits t) (v a);
+    Int.logxor_commutative #(bits t) 0 (v b);
+    Int.logxor_lemma_1 #(bits t) (v b)
 
 let logxor_lemma #t #l a b =
   logxor_lemma_ #t a b;
   v_extensionality (logxor a (logxor a b)) b;
-  assert (a `logxor` (a `logxor` b) == b);
-  (match t with |U1 |U8 |U16 |U32 |U64 |U128 ->
-   UInt.logxor_commutative #(bits t) (v a) (v b)
-   |S8 |S16 |S32 |S64 |S128 -> Int.logxor_commutative #(bits t) (v a) (v b));
-  logxor_lemma_ #t a b;
+  begin
+  match t with 
+  | U1 | U8 | U16 | U32 | U64 | U128 -> UInt.logxor_commutative #(bits t) (v a) (v b)
+  | S8 | S16 | S32 | S64 | S128      -> Int.logxor_commutative #(bits t) (v a) (v b)
+  end;
   v_extensionality (logxor a (logxor b a)) b;
-  assert ((a `logxor` (b `logxor` a)) == b);
-  (match t with |U1 |U8 |U16 |U32 |U64 |U128 ->
-   UInt.logxor_lemma_1 #(bits t) (v a)
-   |S8 |S16 |S32 |S64 |S128 -> Int.logxor_lemma_1 #(bits t) (v a));
-  //UInt.logxor_lemma_1 #(bits t) (v a);
+  begin
+  match t with 
+  | U1 | U8 | U16 | U32 | U64 | U128 -> UInt.logxor_lemma_1 #(bits t) (v a)
+  | S8 | S16 | S32 | S64 | S128      -> Int.logxor_lemma_1 #(bits t) (v a)
+  end;
   v_extensionality (logxor a (mk_int #t #l 0)) a
 
 let logxor_lemma1 #t #l a b =
@@ -459,23 +461,42 @@ let logand #t #l a b =
   | U32  -> UInt32.logand a b
   | U64  -> UInt64.logand a b
   | U128 -> UInt128.logand a b
-  | S8 -> Int8.logand a b
-  | S16 -> Int16.logand a b
-  | S32 -> Int32.logand a b
-  | S64 -> Int64.logand a b
+  | S8   -> Int8.logand a b
+  | S16  -> Int16.logand a b
+  | S32  -> Int32.logand a b
+  | S64  -> Int64.logand a b
   | S128 -> Int128.logand a b
 
 let logand_zeros #t #l a =
-  match t with 
+  match t with
+  | U1 -> assert_norm (u1 0 `logand` zeros U1 l == u1 0 /\ u1 1 `logand` zeros U1 l == u1 0)
   | U8 | U16 | U32 | U64 | U128 -> UInt.logand_lemma_1 #(bits t) (v a)
   | S8 | S16 | S32 | S64 | S128 -> Int.logand_lemma_1 #(bits t) (v a)
 
 let logand_ones #t #l a =
-  match t with 
+  match t with
+  | U1 -> assert_norm (u1 0 `logand` ones U1 l == u1 0 /\ u1 1 `logand` ones U1 l == u1 1)
   | U8 | U16 | U32 | U64 | U128 -> UInt.logand_lemma_2 #(bits t) (v a)
   | S8 | S16 | S32 | S64 | S128 -> Int.logand_lemma_2 #(bits t) (v a)
 
-let logand_spec #t #l a b = ()
+let logand_lemma #t #l a b =
+  logand_zeros #t #l b;  
+  logand_ones #t #l b;
+  match t with
+  | U1 ->
+    assert_norm (u1 0 `logand` zeros U1 l == u1 0 /\ u1 1 `logand` zeros U1 l == u1 0);
+    assert_norm (u1 0 `logand` ones U1 l == u1 0 /\ u1 1 `logand` ones U1 l == u1 1)
+  | U8 | U16 | U32 | U64 | U128 -> UInt.logand_commutative #(bits t) (v a) (v b)
+  | S8 | S16 | S32 | S64 | S128 -> Int.logand_commutative #(bits t) (v a) (v b)
+
+let logand_spec #t #l a b =
+  match t with
+  | U1 -> 
+    assert_norm (u1 0 `logand` u1 0 == u1 0 /\ u1 0 `logand` u1 1 == u1 0);
+    assert_norm (u1 1 `logand` u1 0 == u1 0 /\ u1 1 `logand` u1 1 == u1 1);
+    assert_norm (0 `logand_v #U1` 0 == 0 /\ 0 `logand_v #U1` 1 == 0);
+    assert_norm (1 `logand_v #U1` 0 == 0 /\ 1 `logand_v #U1` 1 == 1)
+  | _ -> ()
 
 let logor #t #l a b =
   match t with
@@ -495,28 +516,26 @@ let logor #t #l a b =
   | S32  -> Int32.logor a b
   | S64  -> Int64.logor a b
   | S128 -> Int128.logor a b
-  
-let logor_spec #t #l a b = ()
 
 #push-options "--max_fuel 1"
 
 let logor_disjoint #t #l a b m =
-  if m > 0 then 
+  if m > 0 then
   begin
     UInt.logor_disjoint #(bits t) (v b) (v a) m;
     UInt.logor_commutative #(bits t) (v b) (v a)
   end
-  else 
+  else
   begin
     UInt.logor_commutative #(bits t) (v a) (v b);
     UInt.logor_lemma_1 #(bits t) (v b)
   end
-  
+
 #pop-options
 
 let lognot #t #l a =
   match t with
-  | U1   -> UInt8.rem (UInt8.lognot a) 0x2uy
+  | U1   -> UInt8.rem (UInt8.lognot a) 2uy
   | U8   -> UInt8.lognot a
   | U16  -> UInt16.lognot a
   | U32  -> UInt32.lognot a
@@ -527,14 +546,7 @@ let lognot #t #l a =
   | S32  -> Int32.lognot a
   | S64  -> Int64.lognot a
   | S128 -> Int128.lognot a
-  
-let shift_right_negative (#n:pos) (a:Int.int_t n{a < 0}) (s:nat) : Tot (Int.int_t n) =
-  let shift_right_negative_vec (#n:pos) (a:BitVector.bv_t n) (s:nat) : Tot (BitVector.bv_t n) =
-  if s >= n then BitVector.ones_vec #n
-  else if s = 0 then a
-  else Seq.append (BitVector.ones_vec #s) (Seq.slice a 0 (n-s))
-  in FStar.Int.from_vec (shift_right_negative_vec #n (FStar.Int.to_vec #n a) s)
-  
+
 let shift_right #t #l a b =
   match t with
   | U1   -> UInt8.shift_right a b
@@ -543,99 +555,78 @@ let shift_right #t #l a b =
   | U32  -> UInt32.shift_right a b
   | U64  -> UInt64.shift_right a b
   | U128 -> UInt128.shift_right a b
-  | S8 -> Int8.shift_arithmetic_right a b
-  | S16 -> Int16.shift_arithmetic_right a b
-  | S32 -> Int32.shift_arithmetic_right a b
-  | S64 -> Int64.shift_arithmetic_right a b
+  | S8   -> Int8.shift_arithmetic_right a b
+  | S16  -> Int16.shift_arithmetic_right a b
+  | S32  -> Int32.shift_arithmetic_right a b
+  | S64  -> Int64.shift_arithmetic_right a b
   | S128 -> Int128.shift_arithmetic_right a b
 
-val shift_right_value_aux_1: #n:pos{n>1} -> a:Int.int_t n -> s:nat{s >= n} ->
+val shift_right_value_aux_1: #n:pos{1 < n} -> a:Int.int_t n -> s:nat{n <= s} ->
   Lemma (Int.shift_arithmetic_right #n a s = a / pow2 s)
 let shift_right_value_aux_1 #n a s =
   pow2_le_compat s n;
-  if a >= 0 then (Int.sign_bit_positive a; assert(a=Int.to_uint a); assert(Int.shift_arithmetic_right #n a s == UInt.shift_right #n a s); UInt.shift_right_value_aux_1 #n a s)
-  else begin
-  Int.sign_bit_negative a;
-  assert (Int.shift_arithmetic_right #n a s = -1);
-  assert (- pow2 s <= a /\ a < 0);
-  small_division_lemma_1 (a+pow2 s) (pow2 s);
-  lemma_div_plus a 1 (pow2 s);
-  assert((a+pow2 s) / pow2 s = 0)
-  end
-  
-val shift_right_value_aux_2: #n:pos -> a:Int.int_t n ->
-  Lemma (Int.shift_arithmetic_right #n a 0 = a / pow2 0)
-let shift_right_value_aux_2 #n a = assert_norm (pow2 0 == 1)
+  if a >= 0 then Int.sign_bit_positive a else Int.sign_bit_negative a
 
-// val append_lemma: #n:pos -> #m:pos -> a:BitVector.bv_t n -> b:BitVector.bv_t m ->
-//   Lemma (Int.from_vec #(n + m) (Seq.append a b) = (Int.from_vec #n a) * pow2 m + (UInt.from_vec #m b))
-// let append_lemma #n #m a b =
-//   let a1 = Int.from_vec #n a in
-//   let a2 = UInt.from_vec #n a in
-//   let b' = UInt.from_vec #m b in
-//   let s1 = Int.from_vec #(n+m) (Seq.append a b) in
-//   let s2 = UInt.from_vec #(n+m) (Seq.append a b) in
-//   admit()
-
-val shift_right_value_aux_0: #n:pos{n > 1} -> a:Int.int_t n ->
-  Lemma (requires True)
-        (ensures Int.shift_arithmetic_right #n a 1 = a / 2)
-
-let shift_right_value_aux_0 #n a =
-  if a >= 0 then begin
-  Int.sign_bit_positive a; 
-  assert(a=Int.to_uint a); 
-  assert(Int.shift_arithmetic_right #n a 1 == UInt.shift_right #n a 1); 
-  UInt.shift_right_value_aux_3 #n a 1
-  end
-  else begin
-  Int.sign_bit_negative a;
-  let a1 = Int.to_vec a in
-  let au = Int.to_uint a in
-  let sar = Int.shift_arithmetic_right #n a 1 in
-  let sar1 = Int.to_vec sar in
-  let sr = UInt.shift_right #n au 1 in
-  let sr1 = UInt.to_vec sr in
-  assert(Seq.equal (Seq.slice sar1 1 n) (Seq.slice sr1 1 n));
-  assert (Seq.equal sar1 (Seq.append (BitVector.ones_vec #1) (Seq.slice sr1 1 n)));
-  UInt.append_lemma #1 #(n-1) (BitVector.ones_vec #1) (Seq.slice sr1 1 n);
-  assert(Seq.equal (Seq.slice a1 0 (n-1)) (Seq.slice sar1 1 n));
-  UInt.slice_left_lemma a1 (n-1);
-  assert (sar + pow2 n = pow2 (n-1) + (au / 2)); 
-  pow2_double_sum (n-1);
-  assert (sar + pow2 (n-1) = (a + pow2 n) / 2);
-  pow2_double_mult (n-1);
-  lemma_div_plus a (pow2 (n-1)) 2;
-  assert (sar = a / 2)
+val shift_right_value_aux_2: #n:pos{1 < n} -> a:Int.int_t n ->
+  Lemma (Int.shift_arithmetic_right #n a 1 = a / 2)
+let shift_right_value_aux_2 #n a =
+  if a >= 0 then 
+    begin
+    Int.sign_bit_positive a;    
+    UInt.shift_right_value_aux_3 #n a 1
+    end
+  else
+    begin
+    Int.sign_bit_negative a;
+    let a1 = Int.to_vec a in
+    let au = Int.to_uint a in
+    let sar = Int.shift_arithmetic_right #n a 1 in
+    let sar1 = Int.to_vec sar in
+    let sr = UInt.shift_right #n au 1 in
+    let sr1 = UInt.to_vec sr in
+    assert (Seq.equal (Seq.slice sar1 1 n) (Seq.slice sr1 1 n));
+    assert (Seq.equal sar1 (Seq.append (BitVector.ones_vec #1) (Seq.slice sr1 1 n)));
+    UInt.append_lemma #1 #(n-1) (BitVector.ones_vec #1) (Seq.slice sr1 1 n);
+    assert (Seq.equal (Seq.slice a1 0 (n-1)) (Seq.slice sar1 1 n));
+    UInt.slice_left_lemma a1 (n-1);
+    assert (sar + pow2 n = pow2 (n-1) + (au / 2));
+    pow2_double_sum (n-1);
+    assert (sar + pow2 (n-1) = (a + pow2 n) / 2);
+    pow2_double_mult (n-1);
+    lemma_div_plus a (pow2 (n-1)) 2;
+    assert (sar = a / 2)
   end
 
 val shift_right_value_aux_3: #n:pos -> a:Int.int_t n -> s:pos{s < n} ->
-  Lemma (requires True)
-        (ensures Int.shift_arithmetic_right #n a s = a / pow2 s)
+  Lemma (ensures Int.shift_arithmetic_right #n a s = a / pow2 s)
         (decreases s)
-        
 let rec shift_right_value_aux_3 #n a s =
-  if s = 1 then shift_right_value_aux_0 #n a
-  else begin
-  let a1 = Int.to_vec a in
-  assert(Seq.equal (BitVector.shift_arithmetic_right_vec #n a1 s) (BitVector.shift_arithmetic_right_vec #n (BitVector.shift_arithmetic_right_vec #n a1 (s-1)) 1));
-  assert (Int.shift_arithmetic_right #n a s = Int.shift_arithmetic_right #n (Int.shift_arithmetic_right #n a (s-1)) 1);
-  shift_right_value_aux_3 #n a (s-1);
-  shift_right_value_aux_0 #n (Int.shift_arithmetic_right #n a (s-1));
-  assert(Int.shift_arithmetic_right #n a s = (a / pow2 (s-1)) / 2);
-  pow2_double_mult (s-1);
-  division_multiplication_lemma a (pow2 (s-1)) 2
-  end
+  if s = 1 then 
+    shift_right_value_aux_2 #n a
+  else 
+    begin
+    let a1 = Int.to_vec a in
+    assert (Seq.equal (BitVector.shift_arithmetic_right_vec #n a1 s)   
+                      (BitVector.shift_arithmetic_right_vec #n
+                         (BitVector.shift_arithmetic_right_vec #n a1 (s-1)) 1));
+    assert (Int.shift_arithmetic_right #n a s = 
+            Int.shift_arithmetic_right #n (Int.shift_arithmetic_right #n a (s-1)) 1);
+    shift_right_value_aux_3 #n a (s-1);
+    shift_right_value_aux_2 #n (Int.shift_arithmetic_right #n a (s-1));
+    assert (Int.shift_arithmetic_right #n a s = (a / pow2 (s-1)) / 2);
+    pow2_double_mult (s-1);
+    division_multiplication_lemma a (pow2 (s-1)) 2
+    end
 
-let shift_right_lemma #t #l a b = 
+let shift_right_lemma #t #l a b =
   match t with
-  |U1 |U8 |U16 |U32 |U64 |U128 -> ()
-  |S8 |S16 |S32 |S64 |S128 -> if (v b >= bits t) then shift_right_value_aux_1 #(bits t) (v a) (v b)
-       else if (v b = 0) then shift_right_value_aux_2 #(bits t) (v a)
-       else shift_right_value_aux_3 #(bits t) (v a) (v b)
-  
-let shift_left_negative (#n:pos) (a:Int.int_t n{a < 0}) (s:nat) : Tot (Int.int_t n) =
-  FStar.Int.from_vec (BitVector.shift_left_vec #n (FStar.Int.to_vec #n a) s)
+  | U1 | U8 | U16 | U32 | U64 | U128 -> ()
+  | S8 | S16 | S32 | S64 | S128 -> 
+    if v b = 0 then ()
+    else if v b >= bits t then 
+      shift_right_value_aux_1 #(bits t) (v a) (v b)
+    else 
+      shift_right_value_aux_3 #(bits t) (v a) (v b)
 
 let shift_left #t #l a b =
   match t with
@@ -645,40 +636,15 @@ let shift_left #t #l a b =
   | U32  -> UInt32.shift_left a b
   | U64  -> UInt64.shift_left a b
   | U128 -> UInt128.shift_left a b
-  | S8 -> if (v a >= 0) then Int8.shift_left a b
-         else Int8.int_to_t (shift_left_negative (Int8.v a) (UInt32.v b))
-  | S16 -> if (v a >= 0) then Int16.shift_left a b
-         else Int16.int_to_t (shift_left_negative (Int16.v a) (UInt32.v b))
-  | S32 -> if (v a >= 0) then Int32.shift_left a b
-         else Int32.int_to_t (shift_left_negative (Int32.v a) (UInt32.v b))
-  | S64 -> if (v a >= 0) then Int64.shift_left a b
-         else Int64.int_to_t (shift_left_negative (Int64.v a) (UInt32.v b))
-  | S128 -> if (v a >= 0) then Int128.shift_left a b
-         else Int128.int_to_t (shift_left_negative (Int128.v a) (UInt32.v b))
+  | S8   -> Int8.shift_left a b           
+  | S16  -> Int16.shift_left a b           
+  | S32  -> Int32.shift_left a b           
+  | S64  -> Int64.shift_left a b           
+  | S128 -> Int128.shift_left a b           
 
 #push-options "--max_fuel 1"
 
-let shift_left_lemma #t #l a b = 
-  match t with
-  |U1 |U8 |U16 |U32 |U64 |U128 -> ()
-  |_ -> let a' = v a in
-       let b' = v b in
-       let n = Int.to_uint a' in
-       let sn = UInt.shift_left #(bits t) n b' in
-       assert(Int.to_vec a' == UInt.to_vec #(bits t) n); 
-       if (a' >= 0) then
-       (assert(a' == n);
-       assert (sn == (n * pow2 b') % pow2 (bits t));
-       ()) else
-       (assert(a'+ pow2 (bits t) == n);
-       assert (sn == (n * pow2 b') % pow2 (bits t));
-       assert (sn == ((a'+pow2 (bits t)) * pow2 b') % pow2 (bits t));
-       distributivity_add_left a' (pow2 (bits t)) (pow2 b');
-       assert (sn == ((a'*pow2 b')+(pow2 (bits t)* pow2 b')) % pow2 (bits t));   
-       swap_mul (pow2 (bits t)) (pow2 b');
-       lemma_mod_plus (a' * pow2 b') (pow2 b') (pow2 (bits t));
-       assert (sn == (a' * pow2 b') % pow2 (bits t));
-       ())
+let shift_left_lemma #t #l a b = ()
 
 let rotate_right #t #l a b =
   logor (shift_right a b) (shift_left a (sub #U32 (size (bits t)) b))
@@ -686,9 +652,10 @@ let rotate_right #t #l a b =
 let rotate_left #t #l a b =
   logor (shift_left a b) (shift_right a (sub #U32 (size (bits t)) b))
 
+// Unused
 inline_for_extraction
-let minus (#t:inttype) (#l:secrecy_level) (a:int_t t l) = 
-  add_mod (lognot a) (mk_int #t #l 1)
+let minus (#t:inttype{unsigned t}) (#l:secrecy_level) (a:int_t t l) =
+  add_mod (lognot a) (mk_int 1)
 
 #pop-options
 
@@ -700,101 +667,88 @@ let eq_mask #t a b =
   | U32  -> UInt32.eq_mask a b
   | U64  -> UInt64.eq_mask a b
   | U128 -> UInt128.eq_mask a b
-  | S8   -> to_i8 #U8 #SEC (UInt8.eq_mask (to_u8 a) (to_u8 b))
-  | S16  -> to_i16 (UInt16.eq_mask (to_u16 a) (to_u16 b))
-  | S32  -> to_i32 (UInt32.eq_mask (to_u32 a) (to_u32 b))
-  | S64  -> to_i64 (UInt64.eq_mask (to_u64 a) (to_u64 b))
-  | S128 -> to_i128 (UInt128.eq_mask (to_u128 a) (to_u128 b))
+  | S8   -> Int.Cast.uint8_to_int8 (UInt8.eq_mask (to_u8 a) (to_u8 b))
+  | S16  -> Int.Cast.uint16_to_int16 (UInt16.eq_mask (to_u16 a) (to_u16 b))
+  | S32  -> Int.Cast.uint32_to_int32 (UInt32.eq_mask (to_u32 a) (to_u32 b))
+  | S64  -> Int.Cast.uint64_to_int64 (UInt64.eq_mask (to_u64 a) (to_u64 b))
 
-let op_At_Percent = Int.op_At_Percent
+val eq_mask_lemma_unsigned: #t:inttype{unsigned t} -> a:int_t t SEC -> b:int_t t SEC -> Lemma
+  (if v a = v b then v (eq_mask a b) == ones_v t
+                else v (eq_mask a b) == 0)
+let eq_mask_lemma_unsigned #t a b =
+  match t with
+  | U1 -> 
+    assert_norm (
+      logxor (u1 0) (u1 0) == u1 0 /\ logxor (u1 0) (u1 1) == u1 1 /\
+      logxor (u1 1) (u1 0) == u1 1 /\ logxor (u1 1) (u1 1) == u1 0 /\
+      lognot (u1 1) == u1 0 /\ lognot (u1 0) == u1 1)      
+  | U8 | U16 | U32 | U64 | U128 -> ()
+
+val eq_mask_lemma_signed: #t:inttype{signed t /\ ~(S128? t)} -> a:int_t t SEC -> b:int_t t SEC -> Lemma
+  (if v a = v b then v (eq_mask a b) == ones_v t
+                else v (eq_mask a b) == 0)
+let eq_mask_lemma_signed #t a b =
+  match t with  
+  | S8 -> 
+    begin
+    assert_norm (pow2 8 = 2 * pow2 7);
+    if 0 <= v a then modulo_lemma (v a) (pow2 8)
+    else 
+      begin
+      modulo_addition_lemma (v a) 1 (pow2 8);
+      modulo_lemma (v a + pow2 8) (pow2 8)
+      end
+    end  
+  | S16 -> 
+    begin
+    assert_norm (pow2 16 = 2 * pow2 15);
+    if 0 <= v a then modulo_lemma (v a) (pow2 16)
+    else 
+      begin
+      modulo_addition_lemma (v a) 1 (pow2 16);
+      modulo_lemma (v a + pow2 16) (pow2 16)
+      end
+    end
+  | S32 -> 
+    begin
+    if 0 <= v a then modulo_lemma (v a) (pow2 32)
+    else 
+      begin
+      modulo_addition_lemma (v a) 1 (pow2 32);
+      modulo_lemma (v a + pow2 32) (pow2 32)
+      end
+    end
+  | S64 -> 
+    begin
+    if 0 <= v a then modulo_lemma (v a) (pow2 64)
+    else 
+      begin
+      modulo_addition_lemma (v a) 1 (pow2 64);
+      modulo_lemma (v a + pow2 64) (pow2 64)
+      end
+    end
 
 let eq_mask_lemma #t a b =
-  match t with
-  | U1 ->
-    begin
-    assert_norm (
-      logxor (u1 0) (u1 0) == u1 0 /\ logxor (u1 1) (u1 1) == u1 0 /\
-      logxor (u1 0) (u1 1) == u1 1 /\ logxor (u1 1) (u1 0) == u1 1 /\
-      lognot (u1 1) == u1 0 /\ lognot (u1 0) == u1 1)
-    end
-  | U8 | U16 | U32 | U64 | U128 -> ()
-  | S8 -> let a' = to_u8 a in let b' = to_u8 b in
-  assert_norm (v a = v b <==> v a' = v b');
-    let m' = UInt8.eq_mask a' b' in
-    assert_norm(v #U8 #SEC m' = 0 ==> v #S8 #SEC (to_i8 m') = 0);
-    assert_norm(v #U8 #SEC m' = ones_v U8 ==> v #S8 #SEC (to_i8 #U8 #SEC m') = -1)
-  | S16 -> let a' = to_u16 a in let b' = to_u16 b in
-    assert (v a = v a' @% pow2 16); assert( v a' = v a % pow2 16);
-    assert (v b = v b' @% pow2 16); assert( v b' = v b % pow2 16);
-    let m' = UInt16.eq_mask a' b' in
-    assert (v a' = v b' ==> v m' = ones_v U16);
-    assert (v a' <> v b' ==> v m' = 0);
-    if (v a = v b) then begin
-      assert (v a' = v b');
-      assert (v m' = ones_v U16);
-      assert (v (to_i16 m') = -1) end
-    else begin
-      assert(v a' <> v b');
-      assert(v m' = 0);
-      assert(v (to_i16 m') = 0) end
-  | S32 -> let a' = to_u32 a in let b' = to_u32 b in
-    assert (v a = v a' @% pow2 32); assert( v a' = v a % pow2 32);
-    assert (v b = v b' @% pow2 32); assert( v b' = v b % pow2 32);
-    let m' = UInt32.eq_mask a' b' in
-    assert (v a' = v b' ==> v m' = ones_v U32);
-    assert (v a' <> v b' ==> v m' = 0);
-    if (v a = v b) then begin
-      assert (v a' = v b');
-      assert (v m' = ones_v U32);
-      assert (v (to_i32 m') = -1) end
-    else begin
-      assert(v a' <> v b');
-      assert(v m' = 0);
-      assert(v (to_i32 m') = 0) end
-  | S64 -> let a' = to_u64 a in let b' = to_u64 b in
-    assert (v a = v a' @% pow2 64); assert( v a' = v a % pow2 64);
-    assert (v b = v b' @% pow2 64); assert( v b' = v b % pow2 64);
-    let m' = UInt64.eq_mask a' b' in
-    assert (v a' = v b' ==> v m' = ones_v U64);
-    assert (v a' <> v b' ==> v m' = 0);
-    if (v a = v b) then begin
-      assert (v a' = v b');
-      assert (v m' = ones_v U64);
-      assert (v (to_i64 m') = -1) end
-    else begin
-      assert(v a' <> v b');
-      assert(v m' = 0);
-      assert(v (to_i64 m') = 0) end
-  | S128 -> let a' = to_u128 a in let b' = to_u128 b in
-    assert (v a = v a' @% pow2 128); assert( v a' = v a % pow2 128);
-    assert (v b = v b' @% pow2 128); assert( v b' = v b % pow2 128);
-    let m' = UInt64.eq_mask a' b' in
-    assert (v a' = v b' ==> v m' = ones_v U64);
-    assert (v a' <> v b' ==> v m' = 0);
-    if (v a = v b) then begin
-      assert (v a' = v b');
-      assert (v m' = ones_v U64);
-      assert (v (to_i128 m') = -1) end
-    else begin
-      assert(v a' <> v b');
-      assert(v m' = 0);
-      assert(v (to_i128 m') = 0) end
+  if signed t then eq_mask_lemma_signed a b
+  else eq_mask_lemma_unsigned a b
 
 let eq_mask_logand_lemma #t a b c =
   eq_mask_lemma a b;
   logand_zeros c;
   logand_ones c;
-  match t with 
-  | U8 | U16 | U32 | U64 | U128 -> UInt.logand_commutative #(bits t) (v (eq_mask a b)) (v c)
-  
+  match t with
+  | U1 | U8 | U16 | U32 | U64 | U128 -> UInt.logand_commutative #(bits t) (v (eq_mask a b)) (v c)
+  | S8 | S16 | S32 | S64 -> Int.logand_commutative #(bits t) (v (eq_mask a b)) (v c)
+
 let neq_mask #t a b = lognot (eq_mask #t a b)
 
-let neq_mask_lemma #t a b = 
+let neq_mask_lemma #t a b =
   match t with
-  | U8 | U16 | U32 | U64 | U128 -> 
+  | U1 -> assert_norm (lognot (u1 1) == u1 0 /\ lognot (u1 0) == u1 1)      
+  | _ ->
     UInt.lognot_lemma_1 #(bits t);
     UInt.lognot_self #(bits t) 0
-  
+
 let gte_mask #t a b =
   match t with
   | U1   -> logor a (lognot b)
@@ -818,11 +772,18 @@ let gte_mask_lemma #t a b =
 let gte_mask_logand_lemma #t a b c =
   logand_zeros c;
   logand_ones c;
-  UInt.logand_commutative #(bits t) (v (gte_mask a b)) (v c)
+  match t with
+  | U1 -> 
+    assert_norm (
+      logor (u1 0) (u1 0) == u1 0 /\ logor (u1 1) (u1 1) == u1 1 /\
+      logor (u1 0) (u1 1) == u1 1 /\ logor (u1 1) (u1 0) == u1 1 /\
+      lognot (u1 1) == u1 0 /\ lognot (u1 0) == u1 1)
+  | _ -> UInt.logand_commutative #(bits t) (v (gte_mask a b)) (v c)
 
 let lt_mask #t a b = lognot (gte_mask a b)
 
 let lt_mask_lemma #t a b =
+  assert_norm (lognot (u1 1) == u1 0 /\ lognot (u1 0) == u1 1);
   UInt.lognot_lemma_1 #(bits t);
   UInt.lognot_self #(bits t) 0
 
@@ -835,46 +796,38 @@ let gt_mask_lemma #t a b =
 let lte_mask #t a b = logor (lt_mask a b) (eq_mask a b)
 
 let lte_mask_lemma #t a b =
-  match t with 
+  match t with
+  | U1 -> 
+    assert_norm (
+      logor (u1 0) (u1 0) == u1 0 /\ logor (u1 1) (u1 1) == u1 1 /\
+      logor (u1 0) (u1 1) == u1 1 /\ logor (u1 1) (u1 0) == u1 1)
   | U8 | U16 | U32 | U64 | U128 ->
-    assume (v a > v b);
-    UInt.logor_lemma_1 #(bits t) (v (lt_mask a b));
-    UInt.logor_lemma_2 #(bits t) (v (eq_mask a b))
- 
- private
-val mod_mask_value: #t:inttype -> #l:secrecy_level -> m:shiftval t ->
+    if v a > v b then
+      UInt.logor_lemma_1 #(bits t) (v (lt_mask a b))
+    else if v a = v b then
+      UInt.logor_lemma_2 #(bits t) (v (lt_mask a b))
+    else
+      UInt.logor_lemma_1 #(bits t) (v (lt_mask a b))
+
+private
+val mod_mask_value: #t:inttype{unsigned t} -> #l:secrecy_level -> m:shiftval t ->
   Lemma (v (mod_mask #t #l m) == pow2 (v m) - 1)
 
-#push-options "--max_fuel 1 "
+#push-options "--max_fuel 1"
 
 let mod_mask_value #t #l m =
   shift_left_lemma (mk_int #t #l 1) m;
-  pow2_double_mult ((bits t) - 1);
-  pow2_le_compat (v m) 0;
+  pow2_double_mult (bits t - 1);
   pow2_lt_compat (bits t) (v m);
   small_modulo_lemma_1 (pow2 (v m)) (pow2 (bits t));
-  small_modulo_lemma_1 ((pow2 (v m)) -1) (pow2 (bits t));
-  assert(v (mod_mask #t #l m) == (((1 * pow2 (v m)) @%. t) - 1) @%. t);
-  match t with
-  |U1 |U8 |U16 |U32 |U64 |U128 -> ()
-  |_ -> if (v m < (bits t) -1) then (pow2_lt_compat (bits t - 1) (v m); assert((1*pow2 (v m))@%. t = pow2 (v m))) else (assert ((1* pow2 (v m)) @%. t = pow2 (v m) - pow2 (bits t)); assert (v m = (bits t) -1); pow2_double_mult ((bits t) -1); assert ((1 * pow2 (v m)) @%. t = - pow2 (v m))) 
+  small_modulo_lemma_1 ((pow2 (v m)) -1) (pow2 (bits t))
 
 let mod_mask_lemma #t #l a m =
   mod_mask_value #t #l m;
-  match t with
-  |U1 |U8 |U16 |U32 |U64 |U128 ->
   if v m = 0 then
     UInt.logand_lemma_1 #(bits t) (v a)
   else
-    UInt.logand_mask #(bits t) (v a) (v m) 
-  |_->
-  if v m = 0 then
-    Int.logand_lemma_1 #(bits t) (v a)
-  else admit() 
-
-#pop-options
-
-let nat_mod_v #m x = x
+    UInt.logand_mask #(bits t) (v a) (v m)
 
 let div #t x y =
   match t with
@@ -883,12 +836,18 @@ let div #t x y =
   | U16 -> UInt16.div x y
   | U32 -> UInt32.div x y
   | U64 -> UInt64.div x y
-  //| S8 -> Int8.div x y
-  //| S16 -> Int16.div x y
-  //| S32 -> Int32.div x y
-  //| S64 -> Int64.div x y
-  
-let div_lemma #t x y = ()
+  | S8  -> Int.pow2_values 8; Int8.div x y  
+  | S16 -> Int.pow2_values 16; Int16.div x y
+  | S32 -> Int.pow2_values 32; Int32.div x y
+  | S64 -> Int.pow2_values 64; Int64.div x y
+
+let div_lemma #t a b =  
+  match t with
+  | U1 | U8 | U16 | U32 | U64 -> ()
+  | S8  -> Int.pow2_values 8
+  | S16 -> Int.pow2_values 16
+  | S32 -> Int.pow2_values 32
+  | S64 -> Int.pow2_values 64
 
 let mod #t x y =
   match t with
@@ -897,105 +856,111 @@ let mod #t x y =
   | U16 -> UInt16.rem x y
   | U32 -> UInt32.rem x y
   | U64 -> UInt64.rem x y
-  //| S8 -> Int8.rem x y
-  //| S16 -> Int16.rem x y
-  //| S32 -> Int32.rem x y
-  //| S64 -> Int64.rem x y
-  
-let mod_lemma #t x y = ()
+  | S8  -> Int.pow2_values 8; Int8.rem x y  
+  | S16 -> Int.pow2_values 16; Int16.rem x y
+  | S32 -> Int.pow2_values 32; Int32.rem x y
+  | S64 -> Int.pow2_values 64; Int64.rem x y
+
+let mod_lemma #t a b =
+  match t with
+  | U1 | U8 | U16 | U32 | U64 -> ()
+  | S8  -> Int.pow2_values 8
+  | S16 -> Int.pow2_values 16
+  | S32 -> Int.pow2_values 32
+  | S64 -> Int.pow2_values 64
 
 let eq #t x y =
   match t with
-  | U1  -> UInt8.eq x y
-  | U8  -> UInt8.eq x y
-  | U16 -> UInt16.eq x y
-  | U32 -> UInt32.eq x y
-  | U64 -> UInt64.eq x y
+  | U1   -> UInt8.eq x y
+  | U8   -> UInt8.eq x y
+  | U16  -> UInt16.eq x y
+  | U32  -> UInt32.eq x y
+  | U64  -> UInt64.eq x y
   | U128 -> UInt128.eq x y
-  | S8  -> Int8.eq x y
-  | S16 -> Int16.eq x y
-  | S32 -> Int32.eq x y
-  | S64 -> Int64.eq x y
+  | S8   -> Int8.eq x y
+  | S16  -> Int16.eq x y
+  | S32  -> Int32.eq x y
+  | S64  -> Int64.eq x y
   | S128 -> Int128.eq x y
 
 let eq_lemma #t x y = ()
 
 let ne #t x y =
   match t with
-  | U1  -> not (UInt8.eq x y)
-  | U8  -> not (UInt8.eq x y)
-  | U16 -> not (UInt16.eq x y)
-  | U32 -> not (UInt32.eq x y)
-  | U64 -> not (UInt64.eq x y)
+  | U1   -> not (UInt8.eq x y)
+  | U8   -> not (UInt8.eq x y)
+  | U16  -> not (UInt16.eq x y)
+  | U32  -> not (UInt32.eq x y)
+  | U64  -> not (UInt64.eq x y)
   | U128 -> not (UInt128.eq x y)
-  | S8  -> not (Int8.eq x y)
-  | S16 -> not (Int16.eq x y)
-  | S32 -> not (Int32.eq x y)
-  | S64 -> not (Int64.eq x y)
+  | S8   -> not (Int8.eq x y)
+  | S16  -> not (Int16.eq x y)
+  | S32  -> not (Int32.eq x y)
+  | S64  -> not (Int64.eq x y)
   | S128 -> not (Int128.eq x y)
-  
+
 let ne_lemma #t x y = ()
 
 let lt #t x y =
   match t with
-  | U1  -> UInt8.lt x y
-  | U8  -> UInt8.lt x y
-  | U16 -> UInt16.lt x y
-  | U32 -> UInt32.lt x y
-  | U64 -> UInt64.lt x y
+  | U1   -> UInt8.lt x y
+  | U8   -> UInt8.lt x y
+  | U16  -> UInt16.lt x y
+  | U32  -> UInt32.lt x y
+  | U64  -> UInt64.lt x y
   | U128 -> UInt128.lt x y
-  | S8  -> Int8.lt x y
-  | S16 -> Int16.lt x y
-  | S32 -> Int32.lt x y
-  | S64 -> Int64.lt x y
+  | S8   -> Int8.lt x y
+  | S16  -> Int16.lt x y
+  | S32  -> Int32.lt x y
+  | S64  -> Int64.lt x y
   | S128 -> Int128.lt x y
-  
+
 let lt_lemma #t x y = ()
 
 let lte #t x y =
   match t with
-  | U1  -> UInt8.lte x y
-  | U8  -> UInt8.lte x y
-  | U16 -> UInt16.lte x y
-  | U32 -> UInt32.lte x y
-  | U64 -> UInt64.lte x y
+  | U1   -> UInt8.lte x y
+  | U8   -> UInt8.lte x y
+  | U16  -> UInt16.lte x y
+  | U32  -> UInt32.lte x y
+  | U64  -> UInt64.lte x y
   | U128 -> UInt128.lte x y
-  | S8  -> Int8.lte x y
-  | S16 -> Int16.lte x y
-  | S32 -> Int32.lte x y
-  | S64 -> Int64.lte x y
+  | S8   -> Int8.lte x y
+  | S16  -> Int16.lte x y
+  | S32  -> Int32.lte x y
+  | S64  -> Int64.lte x y
   | S128 -> Int128.lte x y
-  
+
 let lte_lemma #t x y = ()
 
 let gt #t x y =
   match t with
-  | U1  -> UInt8.gt x y
-  | U8  -> UInt8.gt x y
-  | U16 -> UInt16.gt x y
-  | U32 -> UInt32.gt x y
-  | U64 -> UInt64.gt x y
+  | U1   -> UInt8.gt x y
+  | U8   -> UInt8.gt x y
+  | U16  -> UInt16.gt x y
+  | U32  -> UInt32.gt x y
+  | U64  -> UInt64.gt x y
   | U128 -> UInt128.gt x y
-  | S8  -> Int8.gt x y
-  | S16 -> Int16.gt x y
-  | S32 -> Int32.gt x y
-  | S64 -> Int64.gt x y
+  | S8   -> Int8.gt x y
+  | S16  -> Int16.gt x y
+  | S32  -> Int32.gt x y
+  | S64  -> Int64.gt x y
   | S128 -> Int128.gt x y
-  
+
 let gt_lemma #t x y = ()
 
 let gte #t x y =
   match t with
-  | U1  -> UInt8.gte x y
-  | U8  -> UInt8.gte x y
-  | U16 -> UInt16.gte x y
-  | U32 -> UInt32.gte x y
-  | U64 -> UInt64.gte x y
+  | U1   -> UInt8.gte x y
+  | U8   -> UInt8.gte x y
+  | U16  -> UInt16.gte x y
+  | U32  -> UInt32.gte x y
+  | U64  -> UInt64.gte x y
   | U128 -> UInt128.gte x y
-  | S8  -> Int8.gte x y
-  | S16 -> Int16.gte x y
-  | S32 -> Int32.gte x y
-  | S64 -> Int64.gte x y
+  | S8   -> Int8.gte x y
+  | S16  -> Int16.gte x y
+  | S32  -> Int32.gte x y
+  | S64  -> Int64.gte x y
   | S128 -> Int128.gte x y
-  
+
 let gte_lemma #t x y = ()
